Thanks to Jagannathan \& Wang (1996).

Assume that $\beta_t = \beta_0 + \beta_1 S_t$, where $S$ represents the state of the economy. You can think it as a dummy variable (boom or recession). Now,
$$
\begin{aligned}
		R_{t+1} &= \E_{t}[R_{t+1}] + \beta_t F_{t+1} = \E_{t}[R_{t+1}]  + (\beta_0 + \beta_1 S_t)F_{t+1}\\
				&= \E_t[R_{t+1}] + \beta_0 F_{t+1} + \beta_1 S_t F_{t+1}\\
				&= \E_{t}[R_{t+1}] + \tilde{\beta}\tilde{F}_{t+1},
\end{aligned}
$$
where 
$$
\tilde{\beta} = 	\begin{bmatrix}
\beta_0 & \beta_1
	\end{bmatrix},
\quad\quad
	\tilde{F}_{t+1} = 
	\begin{bmatrix}
		F_{t+1} & S_{t}F_{t+1}
	\end{bmatrix}
$$
